## Theorem
Let $p:\mathcal E\to \mathcal B$ be a [[covering of groupoids]]. Let $\mathcal X$ be a [[groupoid]] and let $f:\mathcal X\to \mathcal B$ be a [[functor]]. Choose a base object $x_0\in\mathcal X$, let $b_0=f(x_0)$, and choose $e_0\in F_{b_0}$. Then there exists a [[functor]]  $g:\mathcal X\to \mathcal E$ such that $g(x_0) = e_0$ and $p\circ g = f$ if and only if $f(\pi(\mathcal X,x_0)) \subset p(\pi(\mathcal E,e_0))$ in $\pi(\mathcal B,b_0)$. When this condition holds, $g$ is unique. 
## Proof
If $g$ exists, because we have chosen $e_0$ to be in the [[fiber]] of $b_0$ under $p$, it must be that we have the inclusion of [[image|images]] $\text{im}(f)\subset \text{im}(p)$. For an object $x$ of $\mathcal X$ and a map $\alpha:x_0\to x$ in $\mathcal X$, let $\tilde\alpha$ be the unique element of the [[star of an object|star]] $\text{St}(e_0)$ such that $p(\tilde\alpha) = f(\alpha)$.  ( #todo why should this be unique?) If $g$ exists, $g(\alpha)$ must be $\tilde \alpha$ and therefore $g(x)$ must be the target $T(f(\alpha))(e_0)$ of $\tilde \alpha$. 

The inclusion $f(\pi(\mathcal X,x_0))\subset p(\pi(\mathcal E, e_0))$ ensure that $T(f(\alpha))(e_0)$ is independent of the choice of $\alpha$, so $g$ is well-defined. Given another map $\alpha':x_0\to x$, the composition $\alpha^{-1}\circ \alpha'$ is even an element of $\pi(\mathcal X,x_0)$. Therefore $$f(\alpha)^{-1}\circ f(\alpha')$ = f(\alpha^{-1}\circ \alpha') = p(\beta)$$ for some $\beta\in \pi(\mathcal E,e_0)$.  Thus $$p(\tilde \alpha\circ \beta) = f(\alpha)\circ p(\beta) = f(\alpha) \circ f(\alpha)^{-1} \circ f(\alpha') = f(\alpha')$$ Thus $\tilde\alpha\circ \beta$ is th eunique element $\tilde\alpha'$ of the [[star of an object|star]] $\text{St}(e_0)$ such that $p(\tilde\alpha')=f(\alpha')$ and its target is the target of $\tilde \alpha$ as required.