## Theorem
Let $f$ be an element of the [[Schwartz space]] for the [[p-adic field]] and let $u$ be a nonzero element of $\mathbb Q_p$. Then the [[Lebesgue integral|integral]] over $\mathbb Q_p$ with respect to the [[Haar measure]] [[Haar measure on additive Qp|on]] $\mathbb Q_p$ of $f(ux)$ is equal to the reciprocal of the $p$-adic [[absolute value]] of $u$ times the [[Lebesgue integral|integral]] over $\mathbb Q_p$ of $f(x)$. That is, $$\int_{\mathbb Q_p}f(ux)\text dx = |u|_p^{-1}\int_{\mathbb Q_p}f(x)\text dx.$$
## Proof
Note that $y$ is in the multiplicative [[left coset|coset]] of the $n$th power of [[curly P]] by $u$ (that is, $y\in u\mathcal P^n$) if and only if its $p$-adic [[absolute value]] is $|y|_p = |u|_p p^{-n}$.  This in turn happens if and only if $|y|_p \leq p^{-n-\text{val}(u)}$ where $\text{val}(u)$ indicates the $p$-adic [[valuation]] of $u$. Finally, this in turn happens if and only if $y \in \mathcal P^{n+\text{val}(u)}$. This means that $u\cdot \mathcal P^n = \mathcal P^{n+\text{val}(u)}$. 

This means that we can compute an [[Lebesgue integral|integral]] to find the [[Haar measure]] [[Haar measure on additive Qp|of]] $u\mathcal P^n$: $$\begin{align*}\int_{u\mathcal P^n}\text dx = \int_{\mathcal P^{n+\text{val}(u)}}\text dx= p^{-n-\text{val}(u)}=p^{-n}|u|_p\end{align*}$$ by [[additive Haar measure of power of curly P is 1/p^n]]. 

By the usual [[change of variables]], we have $$\int_{\mathcal P^k} \text d(u^{-1}x) = \int_{u\mathcal P^k} \text dx = |u|_p\int_{\mathcal P^k}\text dx= |u|_pp^{-n}.$$ From the fact that functions in the [[Schwartz space]] for $\mathbb Q_p$ [[p-adic Schwartz functions are finite linear combinations of characteristic functions of cosets of powers of curly P|are]] finite complex linear combinations of [[characteristic function|characteristic functions]] of additive [[left coset|cosets]] of powers of [[curly P]], there exists $m\in\mathbb Z$ such that any integral $$\int_{\mathbb Q_p}f(ux)\text dx$$ can be written in the form #todo why the hell did sum stop working?$$\int_{\mathbb Q_p} f(ux) \text dx= \int_{\mathbb Q_p}\Sigma_{i=1}^m c_i\chi_{k_i+\mathcal P^m}$$ where $c_i\in\mathbb C$ and $k_i\in\mathbb Q_p$. Then by [[linearity of the integral]], $$\begin{align*}\int_{\mathbb Q_p} f(ux) \text dx&= \int_{\mathbb Q_p} f(x)\text d(u^{-1}x)\\&= \int_{\mathbb Q_p} \left(\Sigma_{i=1}^m c_i\chi_{k_i+\mathcal P^m}(x)\right)\text d(u^{-1}x)\\&= \Sigma c_i\int_{\mathbb Q_p} \chi_{k_i+\mathcal P^m}(x) \text d(u^{-1}x)\\&= \Sigma c_i\int_{k_i+\mathcal P^m}\text d(u^{-1}x)\\&= m\Sigma c_i\int_{\mathcal P^m}\text d(u^{-1}x)\\&= m\Sigma c_i\end{align*}$$ #todo finish