## Theorem
Let $(X,\Sigma, \mu)$ be a [[complete measure space]] and let $\{f_n\}_{n\in\mathbb N}$ be a sequence of real-valued [[measurable function|measurable]] functions [[pointwise convergence|converging pointwise]] [[almost everywhere]] to $f$ dominated by some [[Lebesgue integral|integrable]] function $g$. That is, $|f_n(x)| \leq g(x)$ for all $n \in \mathbb N$ and all $x \in X$. Then $f$ is itself [[Lebesgue integral|integrable]] and $$\lim_{n\to\infty} \int_X |f_n-f|d\mu = 0,$$ which implies that $$\lim_{n\to\infty} \int_X f_n d\mu = \int_X fd\mu.$$
## Proof
Consider the sequence of functions$\{g-f_n\}_{n\in\mathbb N}$. This sequence of functions is nonnegative by construction, and so by [[Fatou's lemma]], $$\liminf_{n\to \infty} g - f_n \geq \int \liminf_{n\to\infty}(g-f_n).$$ By definition of [[limit infimum]], by [[linearity of the integral]], and because [[relation of limit infimum and supremum|the limit supremum is the negative of the limit infimum]], we have $$\liminf_{n\to\infty} \int g-f_n  \int g - \limsup_{n\to\infty}\int f_n \quad\text{and}$$ $$\int\liminf_{n\to\infty} (g-f_n) = \int g - \int \limsup_{n\to\infty} f_n = \int g - \int f.$$ The above inequality implies that $$\limsup_{n\to\infty} f_n \leq \int f.$$ Consider the sequence $\{g+f_n\}_{n\in\mathbb n}$ (still nonnegative) and apply [[Fatou's lemma]] again: $$\liminf \int g+f_n \geq \int \liminf_{n\to\infty} (g+f_n)$$ Then again by [[linearity of the integral]], we have $$\liminf_{n\to\infty} \int g+f_n = \int g + \liminf \int f_n \quad \text{and}$$ $$\int \liminf_{n\to\infty}(g+f_n) = \int g + \int \liminf_{n\to\infty} f_n = \int g + \int f_n.$$ Thus by the above inequality, we have $$\liminf_{n\to\infty} \int f_n \geq \int f.$$ Combining the two inequalities and the definitions of [[limit infimum]] and [[limit supremum|supremum]] yields $$\int f \leq \liminf_{n\to\infty} \int f_n \leq \limsup \int f_n \leq \int f$$  implying that $\lim\limits_{n\to\infty} f_n = \int f$. 
