## Theorem
Let $X,Y \in M_n(\mathbb C)$ be elements of a [[matrix|matrices]]. Then 
1. $e^0 = I$;
2. the [[adjoint of a linear transformation]] (or [[conjugate transpose|Hermitian transpose]]) of the [[exponential of linear transformation|matrix exponential]] is such that $\left(e^X\right)^* = e^{X^*}$;
3. $e^X$ is [[invertible matrix|invertible]] and $\left(e^X\right)^{-1} = e^{-X}$;
4. $e^{(\alpha+\beta)X} = e^{\alpha X}e^{\beta X}$ for all $\alpha,\beta \in \mathbb C$;
5. If $XY=YX$ then $e^{X+Y} = e^Xe^Y= e^Ye^X$;
6. If $C$ is [[invertible matrix|invertible]] then $e^{CXC^{-1}}= Ce^XC^{-1}$.
## Proof
#write_proof [[absolute convergence]]